Weidenbach_Book/WB_More_Refinement.thy
@@ -1139,4 +1139,105 @@ lemma list_rel_mset_rel_imp_same_length: \<open>(a, b) \<in> \<langle>R\<rangle>
   by (auto simp: list_rel_mset_rel_def list_mset_rel_def br_def
       dest: list_rel_imp_same_length)
 
+lemma while_upt_while_direct1:
+  "b \<ge> a \<Longrightarrow> 
+  do {
+    (_,\<sigma>) \<leftarrow> WHILE\<^sub>T (FOREACH_cond c) (\<lambda>x. do {ASSERT (FOREACH_cond c x); FOREACH_body f x}) ([a..<b],\<sigma>);
+    RETURN \<sigma>
+  } \<le> do {
+    (_,\<sigma>) \<leftarrow> WHILE\<^sub>T (\<lambda>(i, x). i < b \<and> c x) (\<lambda>(i, x). do {ASSERT (i < b);  \<sigma>'\<leftarrow>f i x; RETURN (i+1,\<sigma>')
+}) (a,\<sigma>);
+    RETURN \<sigma>
+  }"
+  apply (rewrite at \<open>_ \<le> \<hole>\<close> Down_id_eq[symmetric])
+  apply (refine_vcg WHILET_refine[where R = \<open>{((l, x'), (i::nat, x::'a)). x= x' \<and> i \<le> b \<and> i \<ge> a \<and> l = drop (i-a) [a..<b]}\<close>])
+  subgoal by auto
+  subgoal by (auto simp: FOREACH_cond_def)
+  subgoal by (auto simp: FOREACH_body_def intro!: bind_refine[OF Id_refine])
+  subgoal by auto
+  done
+
+lemma while_upt_while_direct2:
+  "b \<ge> a \<Longrightarrow> 
+  do {
+    (_,\<sigma>) \<leftarrow> WHILE\<^sub>T (FOREACH_cond c) (\<lambda>x. do {ASSERT (FOREACH_cond c x); FOREACH_body f x}) ([a..<b],\<sigma>);
+    RETURN \<sigma>
+  } \<ge> do {
+    (_,\<sigma>) \<leftarrow> WHILE\<^sub>T (\<lambda>(i, x). i < b \<and> c x) (\<lambda>(i, x). do {ASSERT (i < b);  \<sigma>'\<leftarrow>f i x; RETURN (i+1,\<sigma>')
+}) (a,\<sigma>);
+    RETURN \<sigma>
+  }"
+  apply (rewrite at \<open>_ \<le> \<hole>\<close> Down_id_eq[symmetric])
+  apply (refine_vcg WHILET_refine[where R = \<open>{((i::nat, x::'a), (l, x')). x= x' \<and> i \<le> b \<and> i \<ge> a \<and> l = drop (i-a) [a..<b]}\<close>])
+  subgoal by auto
+  subgoal by (auto simp: FOREACH_cond_def)
+  subgoal by (auto simp: FOREACH_body_def intro!: bind_refine[OF Id_refine])
+  subgoal by (auto simp: FOREACH_body_def intro!: bind_refine[OF Id_refine])
+  subgoal by auto
+  done
+
+lemma while_upt_while_direct:
+  "b \<ge> a \<Longrightarrow> 
+  do {
+    (_,\<sigma>) \<leftarrow> WHILE\<^sub>T (FOREACH_cond c) (\<lambda>x. do {ASSERT (FOREACH_cond c x); FOREACH_body f x}) ([a..<b],\<sigma>);
+    RETURN \<sigma>
+  } = do {
+    (_,\<sigma>) \<leftarrow> WHILE\<^sub>T (\<lambda>(i, x). i < b \<and> c x) (\<lambda>(i, x). do {ASSERT (i < b);  \<sigma>'\<leftarrow>f i x; RETURN (i+1,\<sigma>')
+}) (a,\<sigma>);
+    RETURN \<sigma>
+  }"
+  using while_upt_while_direct1[of a b] while_upt_while_direct2[of a b] unfolding order_class.eq_iff by fast
+
+
+lemma while_nfoldli:
+  "do {
+    (_,\<sigma>) \<leftarrow> WHILE\<^sub>T (FOREACH_cond c) (\<lambda>x. do {ASSERT (FOREACH_cond c x); FOREACH_body f x}) (l,\<sigma>);
+    RETURN \<sigma>
+  } \<le> nfoldli l c f \<sigma>"
+  apply (induct l arbitrary: \<sigma>)
+  apply (subst WHILET_unfold)
+  apply (simp add: FOREACH_cond_def)
+
+  apply (subst WHILET_unfold)
+  apply (auto
+    simp: FOREACH_cond_def FOREACH_body_def
+    intro: bind_mono Refine_Basic.bind_mono(1))
+ done
+lemma nfoldli_while: "nfoldli l c f \<sigma>
+          \<le>
+         (WHILE\<^sub>T\<^bsup>I\<^esup>
+           (FOREACH_cond c) (\<lambda>x. do {ASSERT (FOREACH_cond c x); FOREACH_body f x}) (l, \<sigma>) \<bind>
+          (\<lambda>(_, \<sigma>). RETURN \<sigma>))"
+proof (induct l arbitrary: \<sigma>)
+  case Nil thus ?case by (subst WHILEIT_unfold) (auto simp: FOREACH_cond_def)
+next
+  case (Cons x ls)
+  show ?case
+  proof (cases "c \<sigma>")
+    case False thus ?thesis
+      apply (subst WHILEIT_unfold)
+      unfolding FOREACH_cond_def
+      by simp
+  next
+    case [simp]: True
+    from Cons show ?thesis
+      apply (subst WHILEIT_unfold)
+      unfolding FOREACH_cond_def FOREACH_body_def
+      apply clarsimp
+      apply (rule Refine_Basic.bind_mono)
+      apply simp_all
+      done
+  qed
+qed
+
+lemma while_eq_nfoldli: "do {
+    (_,\<sigma>) \<leftarrow> WHILE\<^sub>T (FOREACH_cond c) (\<lambda>x. do {ASSERT (FOREACH_cond c x); FOREACH_body f x}) (l,\<sigma>);
+    RETURN \<sigma>
+  } = nfoldli l c f \<sigma>"
+  apply (rule antisym)
+  apply (rule while_nfoldli)
+  apply (rule order_trans[OF nfoldli_while[where I="\<lambda>_. True"]])
+  apply (simp add: WHILET_def)
+  done
+
 end
